theory/x64Disassembler.thy
@@ -10,221 +10,165 @@ fun x64_disassemble :: "x64_bin \<Rightarrow> x64_asm option" where
 "x64_disassemble (h#t) = (
   if h = 0b10010000 then \<comment> \<open> P2884 `NOP – No Operation` -> `1001 0000` \<close>
     case x64_disassemble t of None \<Rightarrow> None | Some l \<Rightarrow> Some (Pnop # l)
-  else 
-     \<comment> \<open>if h = 0x66 then P518 `Operand-size override prefix is encoded using 66H`  \<close>
-    case t of [] \<Rightarrow> None | h1#[] \<Rightarrow> None | h1#h2#[] \<Rightarrow> None | rex#op#reg#t1 \<Rightarrow> (
-      \<comment> \<open> P2882 `MOV register1 to register2` -> `0100 0R0B : 1000 100w : 11 reg1 reg2` \<close>
-      if op = 0x89 then
-        let r     = unsigned_bitfield_extract_u8 2 1 rex in
-        let b     = unsigned_bitfield_extract_u8 0 1 rex in
-        let modrm = unsigned_bitfield_extract_u8 6 2 reg in
-        let reg1  = unsigned_bitfield_extract_u8 3 3 reg in
-        let reg2  = unsigned_bitfield_extract_u8 0 3 reg in
-        let src   = bitfield_insert_u8 3 1 reg1 r in
-        let dst   = bitfield_insert_u8 3 1 reg2 b in
-          if modrm = 0b11 then (
-            case ireg_of_u8 src of None \<Rightarrow> None | Some src \<Rightarrow> (
-            case ireg_of_u8 dst of None \<Rightarrow> None | Some dst \<Rightarrow> (
-              case x64_disassemble t1 of None \<Rightarrow> None | Some l \<Rightarrow> Some (Pmovq_rr dst src # l) )))
-          else
-            None
-      else if op = 0x01 then
-      \<comment> \<open> P2887 `ADD register1 to register2` -> `0100 WR0B : 0000 000w : 11 reg1 reg2` \<close>
-        let w     = unsigned_bitfield_extract_u8 3 1 rex in
-        let r     = unsigned_bitfield_extract_u8 2 1 rex in
-        let b     = unsigned_bitfield_extract_u8 0 1 rex in
-        let modrm = unsigned_bitfield_extract_u8 6 2 reg in
-        let reg1  = unsigned_bitfield_extract_u8 3 3 reg in
-        let reg2  = unsigned_bitfield_extract_u8 0 3 reg in
-        let src   = bitfield_insert_u8 3 1 reg1 r in
-        let dst   = bitfield_insert_u8 3 1 reg2 b in
-          if modrm = 0b11 then (
-            case ireg_of_u8 src of None \<Rightarrow> None | Some src \<Rightarrow> (
-            case ireg_of_u8 dst of None \<Rightarrow> None | Some dst \<Rightarrow> (
-              if w = 1 then
-                case x64_disassemble t1 of None \<Rightarrow> None | Some l \<Rightarrow> Some (Paddq_rr dst src # l)
-              else 
-                case x64_disassemble t1 of None \<Rightarrow> None | Some l \<Rightarrow> Some (Paddl_rr dst src # l) )))
-          else
-            None
-      else if op = 0x29 then
-      \<comment> \<open> P2891 `SUB register1 from register2` -> `0100 WR0B : 0010 100w : 11 reg1 reg2` \<close> 
-        let w     = unsigned_bitfield_extract_u8 3 1 rex in
-        let r     = unsigned_bitfield_extract_u8 2 1 rex in
-        let b     = unsigned_bitfield_extract_u8 0 1 rex in
-        let modrm = unsigned_bitfield_extract_u8 6 2 reg in
-        let reg1  = unsigned_bitfield_extract_u8 3 3 reg in
-        let reg2  = unsigned_bitfield_extract_u8 0 3 reg in
-        let src   = bitfield_insert_u8 3 1 reg1 r in
-        let dst   = bitfield_insert_u8 3 1 reg2 b in
-          if modrm = 0b11 then (
-            case ireg_of_u8 src of None \<Rightarrow> None | Some src \<Rightarrow> (
-            case ireg_of_u8 dst of None \<Rightarrow> None | Some dst \<Rightarrow> (
-              if w = 1 then
-                case x64_disassemble t1 of None \<Rightarrow> None | Some l \<Rightarrow> Some (Psubq_rr dst src # l)
-              else 
-                case x64_disassemble t1 of None \<Rightarrow> None | Some l \<Rightarrow> Some (Psubl_rr dst src # l) )))
-          else
-            None
-      else if op = 0xf7 then
-      \<comment> \<open> P2884 `NEG  register2`                           -> ` 0100 W00B : 1111 011w : 11011reg` \<close>
-      \<comment> \<open> P2884 `MUL  AL, AX, or EAX with register2`       -> ` 0100 000B : 1111 100w : 11 reg1 reg2` \<close>
-      \<comment> \<open> P2884 `MUL  RAX with qwordregister (to RDX:RAX)` -> ` 0100 100B : 1111 100w : 11 reg1 reg2` \<close>
-      \<comment> \<open> P2884 `IMUL AL, AX, or EAX with register2`       -> ` 0100 000B : 1111 101w : 11 reg1 reg2` \<close>
-      \<comment> \<open> P2880 `IMUL RAX with qwordregister (to RDX:RAX)` -> ` 0100 100B : 1111 101w : 11 reg1 reg2` \<close>
-        let w     = unsigned_bitfield_extract_u8 3 1 rex in
-        let b     = unsigned_bitfield_extract_u8 0 1 rex in
-        let modrm = unsigned_bitfield_extract_u8 6 2 reg in
-        let opex  = unsigned_bitfield_extract_u8 3 3 reg in
-        let reg2  = unsigned_bitfield_extract_u8 0 3 reg in
-        let dst   = bitfield_insert_u8 3 1 reg2 b in
-        if modrm = 0b11 \<and> opex = 0b011 then 
-          case ireg_of_u8 dst of None \<Rightarrow> None | Some dst \<Rightarrow> (
-            if w = 1 then
-              case x64_disassemble t1 of None \<Rightarrow> None | Some l \<Rightarrow> Some (Pnegq dst # l) 
-            else 
-              case x64_disassemble t1 of None \<Rightarrow> None | Some l \<Rightarrow> Some (Pnegl dst # l)) 
-           
-        else if modrm = 0b11 \<and> opex = 0b100 then
-            case ireg_of_u8 dst of None \<Rightarrow> None | Some dst \<Rightarrow> (
-            if w = 1 then
-              case x64_disassemble t1 of None \<Rightarrow> None | Some l \<Rightarrow> Some (Pmulq_r dst # l) 
-            else 
-              case x64_disassemble t1 of None \<Rightarrow> None | Some l \<Rightarrow> Some (Pmull_r dst # l)) 
-        else if modrm = 0b11 \<and> opex = 0b101 then
-            case ireg_of_u8 dst of None \<Rightarrow> None | Some dst \<Rightarrow> (
-            if w = 1 then
-              case x64_disassemble t1 of None \<Rightarrow> None | Some l \<Rightarrow> Some (Pimulq_r dst # l) 
-            else 
-              case x64_disassemble t1 of None \<Rightarrow> None | Some l \<Rightarrow> Some (Pimull_r dst # l)) 
-        else None
-      else if op = 0x09 then
-      \<comment> \<open> P2884 `OR register1 to register2` -> ` 0100 WR0B : 0000 100w : 11 reg1 reg2` \<close>
-        let w     = unsigned_bitfield_extract_u8 3 1 rex in
-        let r     = unsigned_bitfield_extract_u8 2 1 rex in
-        let b     = unsigned_bitfield_extract_u8 0 1 rex in
-        let modrm = unsigned_bitfield_extract_u8 6 2 reg in
-        let reg1  = unsigned_bitfield_extract_u8 3 3 reg in
-        let reg2  = unsigned_bitfield_extract_u8 0 3 reg in
-        let src   = bitfield_insert_u8 3 1 reg1 r in
-        let dst   = bitfield_insert_u8 3 1 reg2 b in
-          if modrm = 0b11 then (
-            case ireg_of_u8 src of None \<Rightarrow> None | Some src \<Rightarrow> (
+  else
+    if h = 0x66 then \<comment> \<open> `16-bit op`  \<close>
+      None
+    else  \<comment> \<open> h is rex  \<close>
+      let w = unsigned_bitfield_extract_u8 3 1 h in
+      let r = unsigned_bitfield_extract_u8 2 1 h in
+      let b = unsigned_bitfield_extract_u8 0 1 h in
+        case t of [] \<Rightarrow> None | h1#[] \<Rightarrow> None | op#reg#t1 \<Rightarrow> (
+          let modrm = unsigned_bitfield_extract_u8 6 2 reg in
+          let reg1  = unsigned_bitfield_extract_u8 3 3 reg in
+          let reg2  = unsigned_bitfield_extract_u8 0 3 reg in
+          let src   = bitfield_insert_u8 3 1 reg1 r in
+          let dst   = bitfield_insert_u8 3 1 reg2 b in
+            \<comment> \<open> P2882 `MOV register1 to register2` -> `0100 0R0B : 1000 100w : 11 reg1 reg2` \<close>
+            if op = 0x89 then
+              if modrm = 0b11 then (
+                case ireg_of_u8 src of None \<Rightarrow> None | Some src \<Rightarrow> (
+                case ireg_of_u8 dst of None \<Rightarrow> None | Some dst \<Rightarrow> (
+                  case x64_disassemble t1 of None \<Rightarrow> None | Some l \<Rightarrow> Some (Pmovq_rr dst src # l) )))
+              else
+                None
+            else if op = 0x01 then
+            \<comment> \<open> P2887 `ADD register1 to register2` -> `0100 WR0B : 0000 000w : 11 reg1 reg2` \<close>
+              if modrm = 0b11 then (
+                case ireg_of_u8 src of None \<Rightarrow> None | Some src \<Rightarrow> (
+                case ireg_of_u8 dst of None \<Rightarrow> None | Some dst \<Rightarrow> (
+                  if w = 1 then
+                    case x64_disassemble t1 of None \<Rightarrow> None | Some l \<Rightarrow> Some (Paddq_rr dst src # l)
+                  else 
+                    case x64_disassemble t1 of None \<Rightarrow> None | Some l \<Rightarrow> Some (Paddl_rr dst src # l) )))
+              else
+                None
+            else if op = 0x29 then
+            \<comment> \<open> P2891 `SUB register1 from register2` -> `0100 WR0B : 0010 100w : 11 reg1 reg2` \<close> 
+              if modrm = 0b11 then (
+                case ireg_of_u8 src of None \<Rightarrow> None | Some src \<Rightarrow> (
+                case ireg_of_u8 dst of None \<Rightarrow> None | Some dst \<Rightarrow> (
+                  if w = 1 then
+                    case x64_disassemble t1 of None \<Rightarrow> None | Some l \<Rightarrow> Some (Psubq_rr dst src # l)
+                  else 
+                    case x64_disassemble t1 of None \<Rightarrow> None | Some l \<Rightarrow> Some (Psubl_rr dst src # l) )))
+              else
+                None
+            else if op = 0xf7 then
+            \<comment> \<open> P2884 `NEG  register2`                           -> ` 0100 W00B : 1111 011w : 11011reg` \<close>
+            \<comment> \<open> P2884 `MUL  AL, AX, or EAX with register2`       -> ` 0100 000B : 1111 100w : 11 reg1 reg2` \<close>
+            \<comment> \<open> P2884 `MUL  RAX with qwordregister (to RDX:RAX)` -> ` 0100 100B : 1111 100w : 11 reg1 reg2` \<close>
+            \<comment> \<open> P2884 `IMUL AL, AX, or EAX with register2`       -> ` 0100 000B : 1111 101w : 11 reg1 reg2` \<close>
+            \<comment> \<open> P2880 `IMUL RAX with qwordregister (to RDX:RAX)` -> ` 0100 100B : 1111 101w : 11 reg1 reg2` \<close>
+            if modrm = 0b11 \<and> reg1 = 0b011 then 
               case ireg_of_u8 dst of None \<Rightarrow> None | Some dst \<Rightarrow> (
                 if w = 1 then
-                  case x64_disassemble t1 of None \<Rightarrow> None | Some l \<Rightarrow> Some (Porq_rr dst src # l) 
+                  case x64_disassemble t1 of None \<Rightarrow> None | Some l \<Rightarrow> Some (Pnegq dst # l) 
                 else 
-                  case x64_disassemble t1 of None \<Rightarrow> None | Some l \<Rightarrow> Some (Porl_rr dst src # l) )))
-          else
-            None
-      else if op = 0x21 then
-      \<comment> \<open> P2876 `AND register1 to register2` -> ` 0100 WR0B : 0000 100w : 11 reg1 reg2` \<close>
-        let w     = unsigned_bitfield_extract_u8 3 1 rex in
-        let r     = unsigned_bitfield_extract_u8 2 1 rex in
-        let b     = unsigned_bitfield_extract_u8 0 1 rex in
-        let modrm = unsigned_bitfield_extract_u8 6 2 reg in
-        let reg1  = unsigned_bitfield_extract_u8 3 3 reg in
-        let reg2  = unsigned_bitfield_extract_u8 0 3 reg in
-        let src   = bitfield_insert_u8 3 1 reg1 r in
-        let dst   = bitfield_insert_u8 3 1 reg2 b in
-          if modrm = 0b11 then (
-            case ireg_of_u8 src of None \<Rightarrow> None | Some src \<Rightarrow> (
-            case ireg_of_u8 dst of None \<Rightarrow> None | Some dst \<Rightarrow> (
-              if w = 1 then
-                case x64_disassemble t1 of None \<Rightarrow> None | Some l \<Rightarrow> Some (Pandq_rr dst src # l)
+                  case x64_disassemble t1 of None \<Rightarrow> None | Some l \<Rightarrow> Some (Pnegl dst # l)) 
+               
+            else if modrm = 0b11 \<and> reg1 = 0b100 then
+                case ireg_of_u8 dst of None \<Rightarrow> None | Some dst \<Rightarrow> (
+                if w = 1 then
+                  case x64_disassemble t1 of None \<Rightarrow> None | Some l \<Rightarrow> Some (Pmulq_r dst # l) 
+                else 
+                  case x64_disassemble t1 of None \<Rightarrow> None | Some l \<Rightarrow> Some (Pmull_r dst # l)) 
+            else if modrm = 0b11 \<and> reg1 = 0b101 then
+                case ireg_of_u8 dst of None \<Rightarrow> None | Some dst \<Rightarrow> (
+                if w = 1 then
+                  case x64_disassemble t1 of None \<Rightarrow> None | Some l \<Rightarrow> Some (Pimulq_r dst # l) 
+                else 
+                  case x64_disassemble t1 of None \<Rightarrow> None | Some l \<Rightarrow> Some (Pimull_r dst # l)) 
+            else None
+          else if op = 0x09 then
+          \<comment> \<open> P2884 `OR register1 to register2` -> ` 0100 WR0B : 0000 100w : 11 reg1 reg2` \<close>
+              if modrm = 0b11 then (
+                case ireg_of_u8 src of None \<Rightarrow> None | Some src \<Rightarrow> (
+                  case ireg_of_u8 dst of None \<Rightarrow> None | Some dst \<Rightarrow> (
+                    if w = 1 then
+                      case x64_disassemble t1 of None \<Rightarrow> None | Some l \<Rightarrow> Some (Porq_rr dst src # l) 
+                    else 
+                      case x64_disassemble t1 of None \<Rightarrow> None | Some l \<Rightarrow> Some (Porl_rr dst src # l) )))
               else
-                case x64_disassemble t1 of None \<Rightarrow> None | Some l \<Rightarrow> Some (Pandl_rr dst src # l))) ) 
-          else
-            None
-       else if op = 0x31 then
-       \<comment> \<open> P2893 `XOR register1 to register2` -> ` 0100 WRXB : 0011 000w : 11 reg1 reg2` \<close>
-        let w     = unsigned_bitfield_extract_u8 3 1 rex in
-        let r     = unsigned_bitfield_extract_u8 2 1 rex in
-        let b     = unsigned_bitfield_extract_u8 0 1 rex in
-        let modrm = unsigned_bitfield_extract_u8 6 2 reg in
-        let reg1  = unsigned_bitfield_extract_u8 3 3 reg in
-        let reg2  = unsigned_bitfield_extract_u8 0 3 reg in
-        let src   = bitfield_insert_u8 3 1 reg1 r in
-        let dst   = bitfield_insert_u8 3 1 reg2 b in
-        if modrm = 0b11 then (
-          case ireg_of_u8 src of None \<Rightarrow> None | Some src \<Rightarrow> (
-          case ireg_of_u8 dst of None \<Rightarrow> None | Some dst \<Rightarrow> (
-            if w = 1 then
-              case x64_disassemble t1 of None \<Rightarrow> None | Some l \<Rightarrow> Some (Pxorq_rr dst src # l)
+                None
+          else if op = 0x21 then
+          \<comment> \<open> P2876 `AND register1 to register2` -> ` 0100 WR0B : 0000 100w : 11 reg1 reg2` \<close>
+              if modrm = 0b11 then (
+                case ireg_of_u8 src of None \<Rightarrow> None | Some src \<Rightarrow> (
+                case ireg_of_u8 dst of None \<Rightarrow> None | Some dst \<Rightarrow> (
+                  if w = 1 then
+                    case x64_disassemble t1 of None \<Rightarrow> None | Some l \<Rightarrow> Some (Pandq_rr dst src # l)
+                  else
+                    case x64_disassemble t1 of None \<Rightarrow> None | Some l \<Rightarrow> Some (Pandl_rr dst src # l))) ) 
+              else
+                None
+           else if op = 0x31 then
+           \<comment> \<open> P2893 `XOR register1 to register2` -> ` 0100 WRXB : 0011 000w : 11 reg1 reg2` \<close>
+            if modrm = 0b11 then (
+              case ireg_of_u8 src of None \<Rightarrow> None | Some src \<Rightarrow> (
+              case ireg_of_u8 dst of None \<Rightarrow> None | Some dst \<Rightarrow> (
+                if w = 1 then
+                  case x64_disassemble t1 of None \<Rightarrow> None | Some l \<Rightarrow> Some (Pxorq_rr dst src # l)
+                else
+                  case x64_disassemble t1 of None \<Rightarrow> None | Some l \<Rightarrow> Some (Pxorl_rr dst src # l))) ) 
             else
-              case x64_disassemble t1 of None \<Rightarrow> None | Some l \<Rightarrow> Some (Pxorl_rr dst src # l))) ) 
-        else
-          None
-       else if op = 0xc1 then
-      \<comment> \<open> P2889 `SHL register by immediate count`      -> ` 0100 000B 1100 000w : 11 100 reg : imm8 ` \<close>
-      \<comment> \<open> P2889 `SHL qwordregister by immediate count` -> ` 0100 100B 1100 000w : 11 100 reg : imm8 ` \<close>
-      \<comment> \<open> P2890 `SHR register by immediate count`      -> ` 0100 000B 1100 000w : 11 101 reg : imm8 ` \<close>
-      \<comment> \<open> P2890 `SHR qwordregister by immediate count` -> ` 0100 100B 1100 000w : 11 101 reg : imm8 ` \<close>
-      \<comment> \<open> P2888 `SAR register by immediate count`      -> ` 0100 000B 1100 000w : 11 111 reg : imm8 ` \<close>
-      \<comment> \<open> P2888 `SAR qwordregister by immediate count` -> ` 0100 100B 1100 000w : 11 111 reg : imm8 ` \<close>
-        case t1 of
-            [] \<Rightarrow> None 
-          | imm#t2 \<Rightarrow> ( 
-              let w = unsigned_bitfield_extract_u8 3 1 rex in
-              let b = unsigned_bitfield_extract_u8 0 1 rex in
-              let modrm = unsigned_bitfield_extract_u8 6 2 reg in
-              let opex = unsigned_bitfield_extract_u8 3 3 reg in
-              let reg2 = unsigned_bitfield_extract_u8 0 3 reg in
-              let dst = bitfield_insert_u8 3 1 reg2 b in
-              if modrm = 0b11 \<and> opex = 0b100 then 
+              None
+           else if op = 0xc1 then
+          \<comment> \<open> P2889 `SHL register by immediate count`      -> ` 0100 000B 1100 000w : 11 100 reg : imm8 ` \<close>
+          \<comment> \<open> P2889 `SHL qwordregister by immediate count` -> ` 0100 100B 1100 000w : 11 100 reg : imm8 ` \<close>
+          \<comment> \<open> P2890 `SHR register by immediate count`      -> ` 0100 000B 1100 000w : 11 101 reg : imm8 ` \<close>
+          \<comment> \<open> P2890 `SHR qwordregister by immediate count` -> ` 0100 100B 1100 000w : 11 101 reg : imm8 ` \<close>
+          \<comment> \<open> P2888 `SAR register by immediate count`      -> ` 0100 000B 1100 000w : 11 111 reg : imm8 ` \<close>
+          \<comment> \<open> P2888 `SAR qwordregister by immediate count` -> ` 0100 100B 1100 000w : 11 111 reg : imm8 ` \<close>
+            case t1 of
+                [] \<Rightarrow> None 
+              | imm#t2 \<Rightarrow> ( 
+                  if modrm = 0b11 \<and> reg1 = 0b100 then 
+                    case ireg_of_u8 dst of None \<Rightarrow> None | Some dst \<Rightarrow> (
+                      if w = 1 then
+                        case x64_disassemble t2 of None \<Rightarrow> None | Some l \<Rightarrow> Some (Pshlq_ri dst imm # l)
+                      else
+                        case x64_disassemble t2 of None \<Rightarrow> None | Some l \<Rightarrow> Some (Pshll_ri dst imm # l))
+                  else if modrm = 0b11 \<and> reg1 = 0b101 then 
+                    case ireg_of_u8 dst of None \<Rightarrow> None | Some dst \<Rightarrow> (
+                      if w = 1 then
+                        case x64_disassemble t2 of None \<Rightarrow> None | Some l \<Rightarrow> Some (Pshrq_ri dst imm # l)
+                      else
+                        case x64_disassemble t2 of None \<Rightarrow> None | Some l \<Rightarrow> Some (Pshrl_ri dst imm # l))
+                  else if modrm = 0b11 \<and> reg1 = 0b111 then 
+                    case ireg_of_u8 dst of None \<Rightarrow> None | Some dst \<Rightarrow> (
+                      if w = 1 then
+                        case x64_disassemble t2 of None \<Rightarrow> None | Some l \<Rightarrow> Some (Psarq_ri dst imm # l)
+                      else
+                        case x64_disassemble t2 of None \<Rightarrow> None | Some l \<Rightarrow> Some (Psarl_ri dst imm # l))
+                  else None)
+          else if op = 0xd3 then
+          \<comment> \<open> P2889 `SHL register by CL`                   -> ` 0100 000B 1100 000w : 11 100 reg ` \<close>
+          \<comment> \<open> P2889 `SHL qwordregister by CL`              -> ` 0100 100B 1100 000w : 11 100 reg ` \<close>
+          \<comment> \<open> P2890 `SHR register by CL`                   -> ` 0100 000B 1100 000w : 11 101 reg ` \<close>
+          \<comment> \<open> P2890 `SHR qwrodregister by CL`              -> ` 0100 100B 1100 000w : 11 101 reg ` \<close>
+          \<comment> \<open> P2888 `SAR register by CL`                   -> ` 0100 000B 1100 000w : 11 111 reg ` \<close>
+          \<comment> \<open> P2888 `SAR qwordregister by CL`              -> ` 0100 100B 1100 000w : 11 111 reg ` \<close>
+            if modrm = 0b11 \<and> reg1 = 0b100 then 
+              case ireg_of_u8 dst of None \<Rightarrow> None | Some dst \<Rightarrow> (
+                if w = 1 then
+                  case x64_disassemble t1 of None \<Rightarrow> None | Some l \<Rightarrow> Some (Pshlq_r dst # l) 
+                else 
+                  case x64_disassemble t1 of None \<Rightarrow> None | Some l \<Rightarrow> Some (Pshll_r dst # l)) 
+            else if modrm = 0b11 \<and> reg1 = 0b101 then
                 case ireg_of_u8 dst of None \<Rightarrow> None | Some dst \<Rightarrow> (
-                  if w = 1 then
-                    case x64_disassemble t2 of None \<Rightarrow> None | Some l \<Rightarrow> Some (Pshlq_ri dst imm # l)
-                  else
-                    case x64_disassemble t2 of None \<Rightarrow> None | Some l \<Rightarrow> Some (Pshll_ri dst imm # l))
-              else if modrm = 0b11 \<and> opex = 0b101 then 
+                if w = 1 then
+                  case x64_disassemble t1 of None \<Rightarrow> None | Some l \<Rightarrow> Some (Pshrq_r dst # l) 
+                else 
+                  case x64_disassemble t1 of None \<Rightarrow> None | Some l \<Rightarrow> Some (Pshrl_r dst # l)) 
+            else if modrm = 0b11 \<and> reg1 = 0b111 then
                 case ireg_of_u8 dst of None \<Rightarrow> None | Some dst \<Rightarrow> (
-                  if w = 1 then
-                    case x64_disassemble t2 of None \<Rightarrow> None | Some l \<Rightarrow> Some (Pshrq_ri dst imm # l)
-                  else
-                    case x64_disassemble t2 of None \<Rightarrow> None | Some l \<Rightarrow> Some (Pshrl_ri dst imm # l))
-              else if modrm = 0b11 \<and> opex = 0b111 then 
-                case ireg_of_u8 dst of None \<Rightarrow> None | Some dst \<Rightarrow> (
-                  if w = 1 then
-                    case x64_disassemble t2 of None \<Rightarrow> None | Some l \<Rightarrow> Some (Psarq_ri dst imm # l)
-                  else
-                    case x64_disassemble t2 of None \<Rightarrow> None | Some l \<Rightarrow> Some (Psarl_ri dst imm # l))
-              else None)
-      else if op = 0xd3 then
-      \<comment> \<open> P2889 `SHL register by CL`                   -> ` 0100 000B 1100 000w : 11 100 reg ` \<close>
-      \<comment> \<open> P2889 `SHL qwordregister by CL`              -> ` 0100 100B 1100 000w : 11 100 reg ` \<close>
-      \<comment> \<open> P2890 `SHR register by CL`                   -> ` 0100 000B 1100 000w : 11 101 reg ` \<close>
-      \<comment> \<open> P2890 `SHR qwrodregister by CL`              -> ` 0100 100B 1100 000w : 11 101 reg ` \<close>
-      \<comment> \<open> P2888 `SAR register by CL`                   -> ` 0100 000B 1100 000w : 11 111 reg ` \<close>
-      \<comment> \<open> P2888 `SAR qwordregister by CL`              -> ` 0100 100B 1100 000w : 11 111 reg ` \<close>
-            let w     = unsigned_bitfield_extract_u8 3 1 rex in
-        let r     = unsigned_bitfield_extract_u8 2 1 rex in
-        let b     = unsigned_bitfield_extract_u8 0 1 rex in
-        let modrm = unsigned_bitfield_extract_u8 6 2 reg in
-        let opex  = unsigned_bitfield_extract_u8 3 3 reg in
-        let reg2  = unsigned_bitfield_extract_u8 0 3 reg in
-        let dst   = bitfield_insert_u8 3 1 reg2 b in
-        if modrm = 0b11 \<and> opex = 0b100 then 
-          case ireg_of_u8 dst of None \<Rightarrow> None | Some dst \<Rightarrow> (
-            if w = 1 then
-              case x64_disassemble t1 of None \<Rightarrow> None | Some l \<Rightarrow> Some (Pshlq_r dst # l) 
-            else 
-              case x64_disassemble t1 of None \<Rightarrow> None | Some l \<Rightarrow> Some (Pshll_r dst # l)) 
-        else if modrm = 0b11 \<and> opex = 0b101 then
-            case ireg_of_u8 dst of None \<Rightarrow> None | Some dst \<Rightarrow> (
-            if w = 1 then
-              case x64_disassemble t1 of None \<Rightarrow> None | Some l \<Rightarrow> Some (Pshrq_r dst # l) 
-            else 
-              case x64_disassemble t1 of None \<Rightarrow> None | Some l \<Rightarrow> Some (Pshrl_r dst # l)) 
-        else if modrm = 0b11 \<and> opex = 0b111 then
-            case ireg_of_u8 dst of None \<Rightarrow> None | Some dst \<Rightarrow> (
-            if w = 1 then
-              case x64_disassemble t1 of None \<Rightarrow> None | Some l \<Rightarrow> Some (Psarq_r dst # l) 
-            else 
-              case x64_disassemble t1 of None \<Rightarrow> None | Some l \<Rightarrow> Some (Psarl_r dst # l)) 
-        else None
-      else 
-        None )
+                if w = 1 then
+                  case x64_disassemble t1 of None \<Rightarrow> None | Some l \<Rightarrow> Some (Psarq_r dst # l) 
+                else 
+                  case x64_disassemble t1 of None \<Rightarrow> None | Some l \<Rightarrow> Some (Psarl_r dst # l)) 
+            else None
+          else 
+            None )
 )"
 
 (*
